MLIR/Dialects/ControlFlowSemantics.lean
@@ -1,18 +1,108 @@
-import MLIR.Dialects.ToyModel
 import MLIR.Semantics.Fitree
-import MLIR.Semantics.Verifier
 import MLIR.Semantics.SSAEnv
 import MLIR.Semantics.InvalidOp
 import MLIR.Util.Metagen
-import MLIR.Util.Reduce
-
 import MLIR.AST
 import MLIR.EDSL
-
-import Lean
-
 open MLIR.AST
 
+/-
+### General semantics
+-/
+
+inductive BlockResult {Gα Gσ Gε} (Gδ: Dialect Gα Gσ Gε)
+| Branch (bb: BBName) (args: List SSAVal)
+| Ret (rets: List (SSAVal × MLIRType Gδ))
+| Next
+
+class Semantics {α σ ε} (δ: Dialect α σ ε) where
+  -- Events modeling the dialect's operations
+  E: Type → Type
+
+  -- Operation semantics function: maps an `Op` to an interaction tree. Usually
+  -- this simply emits an event of `E` and records the return value into the
+  -- environment, and could be automated.
+  semantics_op {Gα Gσ Gε} {Gδ: Dialect Gα Gσ Gε}:
+    Option SSAVal → Op Gδ → Option (Fitree (SSAEnvE Gδ +' E) (BlockResult Gδ))
+
+  -- TODO: Allow a dialects' semantics to specify their terminators along with
+  -- TODO| their branching behavior, instead of hardcoding it for cf
+
+  -- Event handler used when interpreting the operations and running programs.
+  -- This is where most of the semantics and computations take place.
+  -- TODO: Allow dialect handlers to emit events into other dialects
+  handle: E ~> Fitree PVoid
+
+instance {α₁ σ₁ ε₁} {δ₁: Dialect α₁ σ₁ ε₁} {α₂ σ₂ ε₂} {δ₂: Dialect α₂ σ₂ ε₂}
+    [S₁: Semantics δ₁] [S₂: Semantics δ₂]: Semantics (δ₁ + δ₂) where
+  E := S₁.E +' S₂.E
+  semantics_op ret_name op :=
+    (S₁.semantics_op ret_name op).map (.translate Member.inject) <|>
+    (S₂.semantics_op ret_name op).map (.translate Member.inject)
+  handle := Fitree.case_ S₁.handle S₂.handle
+
+def semantics_op! {Gα Gσ Gε} {Gδ: Dialect Gα Gσ Gε} [S: Semantics Gδ]:
+    Option SSAVal → Op Gδ →
+    Fitree (InvalidOpE Gδ +' SSAEnvE Gδ +' S.E) (BlockResult Gδ) :=
+  fun ret op =>
+    match S.semantics_op ret op with
+    | some t => t.translate Member.inject
+    | none => do Fitree.trigger (InvalidOpE.InvalidOp op); return .Next
+
+def semantics_bbstmt {Gα Gσ Gε} {Gδ: Dialect Gα Gσ Gε} [S: Semantics Gδ]:
+    BasicBlockStmt Gδ →
+    Fitree (InvalidOpE Gδ +' SSAEnvE Gδ +' S.E) (BlockResult Gδ)
+| .StmtAssign val _ op => semantics_op! (some val) op
+| .StmtOp op => semantics_op! none op
+
+/-
+### Dialect: `dummy`
+-/
+
+instance dummy: Dialect Void Void (fun x => Unit) where
+  iα := inferInstance
+  iε := inferInstance
+
+inductive DummyE: Type → Type :=
+  | Dummy: DummyE Int
+  | True: DummyE Int
+  | False: DummyE Int
+
+def dummy_semantics_op {Gα Gσ Gε} {Gδ: Dialect Gα Gσ Gε} (ret: Option SSAVal):
+      Op Gδ → Option (Fitree (SSAEnvE Gδ +' DummyE) (BlockResult Gδ))
+  | Op.mk "dummy.dummy" _ _ _ _ (.fn (.tuple []) (.int b)) => some do
+      let i ← Fitree.trigger DummyE.Dummy
+      SSAEnv.set? (δ := Gδ)  (.int b) ret i
+      return BlockResult.Next
+  | Op.mk "dummy.true" _ _ _ _ (.fn (.tuple []) (.int b)) => some do
+      let i ← Fitree.trigger DummyE.True
+      SSAEnv.set? (δ := Gδ) (.int b) ret i
+      return BlockResult.Next
+  | Op.mk "dummy.false" _ _ _ _ (.fn (.tuple []) (.int b)) => some do
+      let i ← Fitree.trigger DummyE.False
+      SSAEnv.set? (δ := Gδ) (.int b) ret i
+      return BlockResult.Next
+  | _ => none
+
+def handle_dummy {E}: DummyE ~> Fitree E :=
+  fun _ e =>
+    match e with
+    | .Dummy => return 42
+    | .True => return 1
+    | .False => return 0
+
+instance: Semantics dummy where
+  E := DummyE
+  semantics_op := dummy_semantics_op
+  handle := handle_dummy
+
+/-
+### Dialect: `cf`
+-/
+
+instance cf: Dialect Void Void (fun x => Unit) where
+  iα := inferInstance
+  iε := inferInstance
 
 set_option hygiene false in
 genInductive ControlFlowOp #[
@@ -29,172 +119,132 @@ genInductive ControlFlowOp #[
   --    ControlFlowOp (τ.eval))
   ]
 
-
-
-inductive BranchType
-| Br (bbname: BBName)
-| Ret
-
-
 -- | interpret branch and conditional branch
-def cf_semantics_op {E: Type -> Type}: Op builtin → Fitree (InvalidOpE +' SSAEnvE builtin +' E) (Option BranchType)
-  | Op.mk "cf.br" [] [bbname] [] _ _ => do
-        return (BranchType.Br bbname)
-  | Op.mk "cf.condbr" [vcond] [bbtrue, bbfalse] _ _ _ => do
-        let condval <- Fitree.trigger $ SSAEnvE.Get (δ := builtin) (.int 32) vcond
-        match condval with
-        | 1 => return (BranchType.Br bbtrue)
-        | _ => return (BranchType.Br bbfalse)
-  | _ => do
-      -- TODO: add error messages.
-      Fitree.trigger InvalidOpE.InvalidOp
-      return Option.none
+def cf_semantics_op (ret_name: Option SSAVal):
+      Op Gδ → Option (Fitree (SSAEnvE Gδ +' PVoid) (BlockResult Gδ))
+  | Op.mk "cf.br" [] [bbname] [] _ _ => some do
+      return BlockResult.Branch bbname []
+  | Op.mk "cf.condbr" [vcond] [bbtrue, bbfalse] _ _ _ => some do
+      let condval <- Fitree.trigger $ SSAEnvE.Get (δ := Gδ) (.int 1) vcond
+      return BlockResult.Branch (if condval != 0 then bbtrue else bbfalse) []
+  | Op.mk "cf.ret" args [] [] _ (.fn (.tuple τs) _) =>
+      if args.length = τs.length then
+        some $ return BlockResult.Ret (List.zip args τs)
+      else none
+  | _ => none
 
+instance: Semantics cf where
+  E := PVoid
+  semantics_op := cf_semantics_op
+  handle := fun _ e => nomatch e
 
+/-
+### More general semantics
+-/
 
--- | TODO: generalize so that each dialect can have its effects.
-def cf_semantics_bbstmt {E: Type -> Type}:
-      BasicBlockStmt builtin → Fitree (InvalidOpE +' SSAEnvE builtin +' E) (Option BranchType)
-  | BasicBlockStmt.StmtAssign val _ op => cf_semantics_op op
-  | BasicBlockStmt.StmtOp op => cf_semantics_op op
-
-
--- | dummy language to check that control flow works correctly.
-def dummy_semantics_op {E: Type -> Type} (ret_name: Option SSAVal):
-      Op builtin → Fitree (InvalidOpE +' SSAEnvE builtin +' E) Unit
-  | Op.mk "dummy.dummy" _ _ _ _ _ =>
-        SSAEnv.set? (δ := builtin) (.int 32) ret_name 42
-  | Op.mk "dummy.true" _ _ _ _ _ =>
-        SSAEnv.set? (δ := builtin) (.int 32) ret_name 1
-  | Op.mk "dummy.false" _ _ _ _ _ =>
-        SSAEnv.set? (δ := builtin) (.int 32) ret_name 0
-  | _ =>
-      -- TODO: add error messages.
-      Fitree.trigger InvalidOpE.InvalidOp
-
-
-def dummy_semantics_bbstmt: BasicBlockStmt builtin ->  Fitree (InvalidOpE +' SSAEnvE builtin +' E) Unit
-| BasicBlockStmt.StmtAssign val _ op => dummy_semantics_op (some val) op
-| BasicBlockStmt.StmtOp op => dummy_semantics_op none op
-
-
--- | TODO: generalize so that each dialect can have its effects.
-@[simp]
-def cf_semantics_bb {E: Type -> Type} (bb: BasicBlock builtin): Fitree (InvalidOpE +' SSAEnvE builtin +' E) (Option BranchType) := do
+-- TODO: Add the basic block arguments and bind them before running the block
+def semantics_bb {Gα Gσ Gε} {Gδ: Dialect Gα Gσ Gε} [S: Semantics Gδ]
+    (bb: BasicBlock Gδ):
+    Fitree (InvalidOpE Gδ +' SSAEnvE Gδ +' S.E) (BlockResult Gδ) := do
+  -- TODO: we assume all statements return BlockResult.Next except the last
   for stmt in bb.stmts.init do
-     dummy_semantics_bbstmt stmt
+    let _ ← semantics_bbstmt stmt
   match bb.stmts.getLast? with
-  | Option.some stmt => cf_semantics_op (stmt.op)
-  | Option.none => return Option.none
+  | some stmt => semantics_bbstmt stmt
+  | none => return BlockResult.Next
 
--- | The semantics of a region are to use up fuel to run the basic block
--- | as many times as necessary.
-def cf_semantics_region_go {E: Type -> Type} (fuel: Nat) (r: Region builtin) (bb: BasicBlock builtin):
-  Fitree (InvalidOpE +' SSAEnvE builtin +' E) (Option BranchType) :=
+def semantics_region_go {Gα Gσ Gε} {Gδ: Dialect Gα Gσ Gε} [S: Semantics Gδ]
+    (fuel: Nat) (r: Region Gδ) (bb: BasicBlock Gδ):
+    Fitree (InvalidOpE Gδ +' SSAEnvE Gδ +' S.E) (BlockResult Gδ) :=
   match fuel with
-  | 0 => return Option.none
-  | Nat.succ fuel' => do
-          -- | TODO: refactor using OptionT transformer
-          match (<- cf_semantics_bb bb) with
-          | Option.none => return Option.none
-          | Option.some (BranchType.Ret) => return (BranchType.Ret)
-          | Option.some (BranchType.Br bbname) =>
-             let bb? := r.getBasicBlock bbname
-             match bb? with
-             | Option.none => return Option.none
-             | Option.some bb' => cf_semantics_region_go fuel' r bb'
+  | 0 => return .Next
+  | fuel' + 1 => do
+      match ← semantics_bb bb with
+        | .Branch bbname args =>
+            -- TODO: Pass the block arguments
+            match r.getBasicBlock bbname with
+            | some bb' => semantics_region_go fuel' r bb'
+            | none => return .Next
+        | .Ret rets => return .Ret rets
+        | .Next => return .Next
 
--- | TODO: write a procedure to determine the return type of a region!
--- | TODO: we need to run some static analysis to find the type of the region o_O ?
-@[simp]
-def cf_semantics_region
-  {E: Type -> Type} (fuel: Nat) (r: Region builtin): Fitree (InvalidOpE +' SSAEnvE builtin +' E) Unit := do
-     let _ <- cf_semantics_region_go fuel r (r.bbs.get! 0)
+-- TODO: Pass region arguments
+-- TODO: Forward region's return type and value
+def semantics_region {Gα Gσ Gε} {Gδ: Dialect Gα Gσ Gε} [S: Semantics Gδ]
+    (fuel: Nat) (r: Region Gδ):
+    Fitree (InvalidOpE Gδ +' SSAEnvE Gδ +' S.E) Unit := do
+  let _ ← semantics_region_go fuel r (r.bbs.get! 0)
 
-@[simp]
-def run_cf (t: Fitree (InvalidOpE +' SSAEnvE builtin +' PVoid) Unit) (env: SSAEnv builtin):
-    Fitree PVoid ((Unit × String) × SSAEnv builtin) :=
-  let x := interp_ssa_logged (interp_invalid t sorry)
-  let y := x.run
-  let z := y env
-  z
+def semantics_run {Gα Gσ Gε} {Gδ: Dialect Gα Gσ Gε} [S: Semantics Gδ] {R}
+    (t: Fitree (InvalidOpE Gδ +' SSAEnvE Gδ +' S.E) R) (env: SSAEnv Gδ):
+    R × SSAEnv Gδ :=
+  let t := interp_invalid! t
+  let t := interp_ssa t env
+  let t := interp S.handle t
+  t.run
 
+def semantics_run_logged {Gα Gσ Gε} {Gδ: Dialect Gα Gσ Gε} [S: Semantics Gδ]
+    {R} (t: Fitree (InvalidOpE Gδ +' SSAEnvE Gδ +' S.E) R) (env: SSAEnv Gδ):
+    (R × String) × SSAEnv Gδ :=
+  let t := interp_invalid! t
+  let t := (interp_ssa_logged t).run env
+  let t := interp S.handle t
+  t.run
 
 /-
 ### Examples and testing
 -/
 
 -- #reduce spins on the dialect coercion because it's mutually inductive, even
--- with skipProofs := true (why?!), so define it as builtin directly
-def dummy_stmt: BasicBlockStmt builtin := [mlir_bb_stmt|
-  %dummy = "dummy.dummy"() : ()
+-- with skipProofs := true (why?!), so define it directly in the dummy dialect
+def dummy_stmt: BasicBlockStmt dummy := [mlir_bb_stmt|
+  %dummy = "dummy.dummy"() : () -> i32
 ]
+#reduce semantics_bbstmt dummy_stmt
 
-#reduce (skipProofs := true)
-  dummy_semantics_bbstmt dummy_stmt
-
-
-def true_stmt: BasicBlockStmt builtin := [mlir_bb_stmt|
-  %true = "dummy.true"() : ()
+def true_stmt: BasicBlockStmt dummy := [mlir_bb_stmt|
+  %true = "dummy.true"() : () -> i1
 ]
+#reduce semantics_bbstmt true_stmt
 
-#reduce (skipProofs := true)
-  dummy_semantics_bbstmt true_stmt
-
-
-def false_stmt: BasicBlockStmt builtin := [mlir_bb_stmt|
-  %false = "dummy.false"() : ()
+def false_stmt: BasicBlockStmt dummy := [mlir_bb_stmt|
+  %false = "dummy.false"() : () -> i1
 ]
-#reduce (skipProofs := true)
-  dummy_semantics_bbstmt false_stmt
+#reduce semantics_bbstmt false_stmt
 
+def run_dummy_cf_region: Region (dummy + cf) → String := fun r =>
+  semantics_run_logged (semantics_region 99 r) SSAEnv.empty |>.fst |>.snd
 
-def branch_to_true_region: Region builtin := [mlir_region| {
+def ex_branch_true: Region dummy := [mlir_region| {
   ^entry:
-    %x = "dummy.true"() : ()
+    %x = "dummy.true"() : () -> i1
     "cf.condbr"(%x) [^bbtrue, ^bbfalse] : ()
 
   ^bbtrue:
-    %y = "dummy.dummy" () : ()
-    "ret" () : ()
+    %y = "dummy.dummy" () : () -> i32
+    "cf.ret" () : ()
 
   ^bbfalse:
-    %z = "dummy.dummy" () : ()
-    "ret" () : ()
-
+    %z = "dummy.dummy" () : () -> i32
+    "cf.ret" () : ()
 }]
 
-#eval branch_to_true_region
+#eval ex_branch_true
+#eval run_dummy_cf_region ex_branch_true
 
-def run_branch_true : String :=
-  let x := run_cf (cf_semantics_region 5 branch_to_true_region) SSAEnv.empty
-  let y := Fitree.run x
-  y.fst.snd
-
-#eval run_branch_true
-
-
-def branch_to_false_region := [mlir_region| {
+def ex_branch_false := [mlir_region| {
   ^entry:
-    %x = "dummy.false"() : ()
+    %x = "dummy.false"() : () -> i1
     "cf.condbr"(%x) [^bbtrue, ^bbfalse] : ()
-    -- "cf.br" () [^bbtrue] : ()
 
   ^bbtrue:
-    %y = "dummy.dummy" () : ()
+    %y = "dummy.dummy" () : () -> i32
     "ret" () : ()
 
   ^bbfalse:
-    %z = "dummy.dummy" () : ()
+    %z = "dummy.dummy" () : () -> i32
     "ret" () : ()
-
 }]
 
-#eval branch_to_false_region
-
-def run_branch_false : String :=
-  let x := run_cf (cf_semantics_region 100 branch_to_false_region) SSAEnv.empty
-  let y := Fitree.run x
-  y.fst.snd
-
-#eval run_branch_false
+#eval ex_branch_false
+#eval run_dummy_cf_region ex_branch_false
